Broken Hamster

Validation/Dafny/Hamster.dfy
@@ -1,54 +1,101 @@
 trait PointT {
-  var x: real
-  var y: real
-  method clone() returns (p: PointT)
+  var x: int
+  var y: int
+
+  method Clone() 
+    returns (p: PointT) 
     ensures fresh(p)
-  function method Equal(p: PointT): bool reads this, p ensures this == p ==> this.Equal(p)
+
+  function method Equal(p: PointT): 
+    bool reads this, p ensures this == p ==> this.Equal(p)
 }
 
 class Point extends PointT
 {
-  function method Equal(p: PointT): bool reads this, p ensures this == p ==> this.Equal(p)
-  { this.x == p.x && this.y == p.y }
 
-  constructor (xx: real, yy: real) { x := xx; y := yy;  }
-
-  method clone() returns (p: PointT)
-    ensures fresh(p) {
+  constructor (xx: int, yy: int) { x := xx; y := yy;  }
+  function method Equal(p: PointT): bool 
+    reads this, p ensures this == p ==> this.Equal(p) 
+  {
+    this.x == p.x && this.y == p.y 
+  }
+  method Clone() returns (p: PointT) ensures fresh(p) 
+  {
       p := new Point(x, y);
   }
 }
 
-method Assume(b: bool) 
-  decreases *
-  ensures b {
-  if !b {
+method {:opaque} Assume(b: bool) decreases * ensures b 
+{
+  if !b 
+  {
     print "Asssumption failed!";
     while (true) decreases * { }
   }
 }
-class {:autocontracts} Hamster {
+
+class Hamster {
   var pos: PointT
-  constructor (p: PointT)
-    decreases *
-  { 
-    var p2 := p.clone();
-    this.pos := p2;
-    var b := ValidF(p); 
-    Assume(b);
-  }
-  static function method ValidF(pos: PointT): bool reads pos { !pos.Equal(pos) }
-  function method Valid(): bool reads this.pos { ValidF(this.pos) }
+  constructor (p: PointT) { this.pos := p; }
 }
 
+type Path = array<PointT>
+class {:autocontracts} Cage
+{
+  var path: Path
+  var h: Hamster
 
-/*class Cage {
-  var path: seq<PointT>;
-}*/
+  constructor (h: Hamster, path: Path) decreases *
+  {
+    this.h := new Hamster(h.pos);   
+    this.path := new PointT[path.Length](
+      (i : nat) reads path requires i < path.Length => path[i]
+    );
+    new;
+    Assume(this.Valid());
+  }
+
+  function method Valid(): bool 
+    reads this, this.h, this.h.pos, this.path, this.path[..] 
+    reads this, Repr
+  {
+    exists p : PointT | p in this.path[..] :: p.Equal(this.h.pos)
+  }
+
+  method Move()
+    decreases *
+    modifies this, this.h, this.h.pos
+  { 
+		var index := 1;
+		while index <= this.path.Length && !this.path[index - 1].Equal(this.h.pos) { 
+      index := index + 1;
+    }
+
+    //assert this.path.Length > 0;
+		this.h.pos := this.path[index % this.path.Length];
+    Assume(this.Valid());
+	}
+}
+
 method Main() 
   decreases *
 {
   print "hello, Dafny\n";
-  var p := new Point(0.0, 1.0);
-  var x := new Hamster(p);
+  var p0 := new Point(0, 0);
+  var p1 := new Point(2, 2);
+  var p2 := new Point(0, 0);
+  var pl := new PointT[3][p0, p1, p2];
+
+  var ph := new Point(0, 0);
+  var h := new Hamster(ph);
+  var c := new Cage(h, pl);
+
+//  Assume(c.h.pos.x == 0 && c.h.pos.y == 0);
+  c.Move();
+ // Assume(c.h.pos.x == 2 && c.h.pos.y == 2);
+  c.Move();
+ // Assume(c.h.pos.x == 0 && c.h.pos.y == 0);
+  c.Move();
+// Assume(c.h.pos.x == 2 && c.h.pos.y == 2);
+  //PlayWith(c);
 }
